vstep/vst_hints.v
@@ -3,6 +3,35 @@ From diaframe Require Import defs proofmode_base.
 Require Import VST.concurrency.conclib.
 Require Import VST.concurrency.lock_specs.
 
+Section SPECS.
+Context `{!VSTGS OK_ty Σ}.
+Context {LI : lock_impl}.
+
+Notation InvType := Mpred.
+
+  Program Definition release_spec_simple2 :=
+    TYPE (ProdType (ConstType _) InvType)
+    WITH sh : _, h : _, R : _
+    PRE [ tptr t_lock ]
+       PROP (ExclusiveProp R)
+       PARAMS (ptr_of h)
+       SEP (lock_inv sh h R; R)
+    POST [ tvoid ]
+       PROP ()
+       LOCAL ()
+       SEP (lock_inv sh h R).
+  Next Obligation.
+  Admitted.
+  Next Obligation.
+  Admitted.
+
+  Lemma release_simple2 : funspec_sub lock_specs.release_spec release_spec_simple2.
+  Proof.
+    Admitted.
+End SPECS.
+
+
+
 Section CONC_HINTS.
 Context `{!VSTGS unit Σ}.
 Global Instance lock_prop_hint {prop:bi} (P:prop):
